\documentclass[a4paper,12pt]{article}
\begin{document}
Calculating
\begin{math}
	(( sin (x)  + 3 \cdot y) \cdot x + 12)'
\end{math}
 $ = Calculating
\begin{math}
	(( sin (x)  + 3 \cdot y) \cdot x)'
\end{math}
 $ = $\\
Calculating
\begin{math}
	(( sin (x)  + 3 \cdot y))'
\end{math}
 $ = Calculating
\begin{math}
	( sin (x) )'
\end{math}
 $ = $\\
Calculating
\begin{math}
	(x)'
\end{math}
 $ = 1\\
Calculating
\begin{math}
	(3 \cdot y)'
\end{math}
 $ = $\\
Calculating
\begin{math}
	(3)'
\end{math}
 $ = 0\\
Calculating
\begin{math}
	(y)'
\end{math}
 $ = \frac{dy}{dx}$\\
Calculating
\begin{math}
	(x)'
\end{math}
 $ = 1\\
Calculating
\begin{math}
	(12)'
\end{math}
 $ = 0\\
\end{document}
